# Proof Analysis Report

**Generated:** 2026-02-25 01:59:43

## Raw Code

```lean
import Mathlib
set_option maxHeartbeats 0
open BigOperators Real Nat Topology Rat
lemma aime_1983_p3_1_1
    (f : ℝ → ℝ)
    (h₀ : ∀ x : ℝ,
        f x =
        x ^ 2 + (18 * x + 30) - 2 * √(x ^ 2 + 18 * x + 45))
    (h₁ : Fintype (↑(f ⁻¹' {0}) : Type)) :
    ∏ x ∈ (f ⁻¹' {0}).toFinset, x = 20 := by
  have h2 : ∀ x : ℝ, f x = 0 ↔ x = -9 + √61 ∨ x = -9 - √61 := by
    intro x
    constructor
    · -- Assume f(x) = 0, prove x = -9 ± √61
        intro hx
        have hfx : f x = x ^ 2 + (18 * x + 30) - 2 * √(x ^ 2 + 18 * x + 45) := h₀ x
        rw [hfx] at hx
        have h_eq : x ^ 2 + (18 * x + 30) - 2 * √(x ^ 2 + 18 * x + 45) = 0 := hx
        have h1 : 2 * √(x ^ 2 + 18 * x + 45) = x ^ 2 + 18 * x + 30 := by linarith
        have h2 : x ^ 2 + 18 * x + 45 ≥ 0 := by
            nlinarith [Real.sqrt_nonneg (x ^ 2 + 18 * x + 45)]
        have h3 : √(x ^ 2 + 18 * x + 45) ≥ 0 := Real.sqrt_nonneg (x ^ 2 + 18 * x + 45)
        have h4 : x ^ 2 + 18 * x + 30 ≥ 0 := by nlinarith
        have h5 : x ^ 2 + 18 * x + 30 = 2 * √(x ^ 2 + 18 * x + 45) := by linarith
        have h6 : (x ^ 2 + 18 * x + 30) ^ 2 = 4 * (x ^ 2 + 18 * x + 45) := by
            have hsq : (2 * √(x ^ 2 + 18 * x + 45)) ^ 2 = 4 * (x ^ 2 + 18 * x + 45) := by
                calc
                    (2 * √(x ^ 2 + 18 * x + 45)) ^ 2 = 4 * (√(x ^ 2 + 18 * x + 45) ^ 2) := by ring
                    _ = 4 * (x ^ 2 + 18 * x + 45) := by rw [Real.sq_sqrt h2]
            rw [← h5] at hsq
            nlinarith
        have h7 : (x - (-9 + √61)) * (x - (-9 - √61)) = 0 := by
            ring_nf
            nlinarith [h6, Real.sq_sqrt (show 0 ≤ 61 by norm_num : (61 : ℝ) ≥ 0)]
        cases' (mul_eq_zero.mp h7) with h8 h9
        · left
          linarith
        · right
          linarith
    · -- Assume x = -9 ± √61, prove f(x) = 0
        rintro (h | h)
        · rw [h]
          have h1 : √61 > 0 := Real.sqrt_pos.mpr (by norm_num : (61 : ℝ) > 0)
          have h2 : (-9 + √61) ^ 2 + 18 * (-9 + √61) + 30 = 2 * √61 * (-9 + √61) := by
            ring_nf
            nlinarith [Real.sq_sqrt (show 0 ≤ 61 by norm_num : (61 : ℝ) ≥ 0)]
          have h3 : √((-9 + √61) ^ 2 + 18 * (-9 + √61) + 45) = √61 := by
            rw [h2]
            rw [Real.sqrt_mul (by linarith)]
            have h4 : √61 * √61 = 61 := by
              rw [Real.mul_self_sqrt (by linarith)]
            nlinarith
          rw [h3]
          ring
        · rw [h]
          have h1 : √61 > 0 := Real.sqrt_pos.mpr (by norm_num : (61 : ℝ) > 0)
          have h2 : (-9 - √61) ^ 2 + 18 * (-9 - √61) + 30 = -2 * √61 * (-9 - √61) := by
            ring_nf
            nlinarith [Real.sq_sqrt (show 0 ≤ 61 by norm_num : (61 : ℝ) ≥ 0)]
          have h3 : √((-9 - √61) ^ 2 + 18 * (-9 - √61) + 45) = √61 := by
            rw [h2]
            rw [Real.sqrt_mul (by linarith)]
            have h4 : √61 * √61 = 61 := by
              rw [Real.mul_self_sqrt (by linarith)]
            nlinarith
          rw [h3]
          ring
  have h3 : (f ⁻¹' {0} : Set ℝ) = {(-9 + √61), (-9 - √61)} := by
    ext x
    simp [h2]
    <;> constructor
    · intro hx
      exact hx
    · rintro (rfl | rfl)
      · left; linarith
      · right; linarith
  rw [h3]
  simp [Finset.prod_pair]
  have h4 : (-9 + √61) * (-9 - √61) = 20 := by
    calc
        (-9 + √61) * (-9 - √61) = (-9) ^ 2 - (√61) ^ 2 := by ring
        _ = 81 - 61 := by norm_num [Real.sq_sqrt]
        _ = 20 := by norm_num
  exact h4

```

## Corrected Code

```lean
import Mathlib
set_option maxHeartbeats 0
open BigOperators Real Nat Topology Rat
lemma aime_1983_p3_1_1
    (f : ℝ → ℝ)
    (h₀ : ∀ x : ℝ,
        f x =
        x ^ 2 + (18 * x + 30) - 2 * √(x ^ 2 + 18 * x + 45))
    (h₁ : Fintype (↑(f ⁻¹' {0}) : Type)) :
    ∏ x ∈ (f ⁻¹' {0}).toFinset, x = 20 := by
  have h2 : ∀ x : ℝ, f x = 0 ↔ x = -9 + √61 ∨ x = -9 - √61 := by
    intro x
    constructor
    · -- Assume f(x) = 0, prove x = -9 ± √61
        intro hx
        have hfx : f x = x ^ 2 + (18 * x + 30) - 2 * √(x ^ 2 + 18 * x + 45)  := by
          h₀ x
        rw [hfx] at hx
        have h_eq : x ^ 2 + (18 * x + 30) - 2 * √(x ^ 2 + 18 * x + 45) = 0  := by
          hx
        have h1 : 2 * √(x ^ 2 + 18 * x + 45) = x ^ 2 + 18 * x + 30  := by
          linarith
        have h2 : x ^ 2 + 18 * x + 45 ≥ 0 := by
            nlinarith [Real.sqrt_nonneg (x ^ 2 + 18 * x + 45)]
        have h3 : √(x ^ 2 + 18 * x + 45) ≥ 0  := by
          Real.sqrt_nonneg (x ^ 2 + 18 * x + 45)
        have h4 : x ^ 2 + 18 * x + 30 ≥ 0  := by
          nlinarith
        have h5 : x ^ 2 + 18 * x + 30 = 2 * √(x ^ 2 + 18 * x + 45)  := by
          linarith
        have h6 : (x ^ 2 + 18 * x + 30) ^ 2 = 4 * (x ^ 2 + 18 * x + 45) := by
            have hsq : (2 * √(x ^ 2 + 18 * x + 45)) ^ 2 = 4 * (x ^ 2 + 18 * x + 45) := by
                    (2 * √(x ^ 2 + 18 * x + 45)) ^ 2 = 4 * (√(x ^ 2 + 18 * x + 45) ^ 2) := by ring
                    _ = 4 * (x ^ 2 + 18 * x + 45) := by rw [Real.sq_sqrt h2]
            rw [← h5] at hsq
            nlinarith
        have h7 : (x - (-9 + √61)) * (x - (-9 - √61)) = 0 := by
            ring_nf
            nlinarith [h6, Real.sq_sqrt (show 0 ≤ 61 by norm_num : (61 : ℝ) ≥ 0)]
        cases' (mul_eq_zero.mp h7) with h8 h9
        · left
          linarith
        · right
          linarith
    · -- Assume x = -9 ± √61, prove f(x) = 0
        rintro (h | h)
        · rw [h]
          have h1 : √61 > 0  := by
            Real.sqrt_pos.mpr (by norm_num : (61 : ℝ) > 0)
          have h2 : (-9 + √61) ^ 2 + 18 * (-9 + √61) + 30 = 2 * √61 * (-9 + √61) := by
            ring_nf
            nlinarith [Real.sq_sqrt (show 0 ≤ 61 by norm_num : (61 : ℝ) ≥ 0)]
          have h3 : √((-9 + √61) ^ 2 + 18 * (-9 + √61) + 45) = √61 := by
            rw [h2]
            rw [Real.sqrt_mul (by linarith)]
            have h4 : √61 * √61 = 61 := by
              rw [Real.mul_self_sqrt (by linarith)]
            nlinarith
          rw [h3]
          ring
        · rw [h]
          have h1 : √61 > 0  := by
            Real.sqrt_pos.mpr (by norm_num : (61 : ℝ) > 0)
          have h2 : (-9 - √61) ^ 2 + 18 * (-9 - √61) + 30 = -2 * √61 * (-9 - √61) := by
            ring_nf
            nlinarith [Real.sq_sqrt (show 0 ≤ 61 by norm_num : (61 : ℝ) ≥ 0)]
          have h3 : √((-9 - √61) ^ 2 + 18 * (-9 - √61) + 45) = √61 := by
            rw [h2]
            rw [Real.sqrt_mul (by linarith)]
            have h4 : √61 * √61 = 61 := by
              rw [Real.mul_self_sqrt (by linarith)]
            nlinarith
          rw [h3]
          ring
  have h3 : (f ⁻¹' {0} : Set ℝ) = {(-9 + √61), (-9 - √61)} := by
    ext x
    simp [h2]
    <;> constructor
    · intro hx
      exact hx
    · rintro (rfl | rfl)
      · left; linarith
      · right; linarith
  rw [h3]
  simp [Finset.prod_pair]
  have h4 : (-9 + √61) * (-9 - √61) = 20 := by
        (-9 + √61) * (-9 - √61) = (-9) ^ 2 - (√61) ^ 2 := by ring
        _ = 81 - 61 := by norm_num [Real.sq_sqrt]
        _ = 20 := by norm_num
  exact h4
```

## Initial Verification

**Status:** ❌ FAIL

### Errors

```bash
- **Line 17:** unknown tactic
- **Line 16:** unsolved goals
f : ℝ → ℝ
h₀ : ∀ (x : ℝ), f x = x ^ 2 + (18 * x + 30) - 2 * √(x ^ 2 + 18 * x + 45)
h₁ : Fintype ↑(f ⁻¹' {0})
x : ℝ
hx : f x = 0
⊢ f x = x ^ 2 + (18 * x + 30) - 2 * √(x ^ 2 + 18 * x + 45)
- **Line 14:** unsolved goals
case mp
f : ℝ → ℝ
h₀ : ∀ (x : ℝ), f x = x ^ 2 + (18 * x + 30) - 2 * √(x ^ 2 + 18 * x + 45)
h₁ : Fintype ↑(f ⁻¹' {0})
x : ℝ
hx : f x = 0
hfx : f x = x ^ 2 + (18 * x + 30) - 2 * √(x ^ 2 + 18 * x + 45)
⊢ x = -9 + √61 ∨ x = -9 - √61
- **Line 11:** unsolved goals
case mpr
f : ℝ → ℝ
h₀ : ∀ (x : ℝ), f x = x ^ 2 + (18 * x + 30) - 2 * √(x ^ 2 + 18 * x + 45)
h₁ : Fintype ↑(f ⁻¹' {0})
x : ℝ
⊢ x = -9 + √61 ∨ x = -9 - √61 → f x = 0
- **Line 10:** unsolved goals
f : ℝ → ℝ
h₀ : ∀ (x : ℝ), f x = x ^ 2 + (18 * x + 30) - 2 * √(x ^ 2 + 18 * x + 45)
h₁ : Fintype ↑(f ⁻¹' {0})
h2 : ∀ (x : ℝ), f x = 0 ↔ x = -9 + √61 ∨ x = -9 - √61
⊢ ∏ x ∈ (f ⁻¹' {0}).toFinset, x = 20

```

## Sorrification Process

### Sorrified Result

```lean
import Mathlib
set_option maxHeartbeats 0
open BigOperators Real Nat Topology Rat
lemma aime_1983_p3_1_1
    (f : ℝ → ℝ)
    (h₀ : ∀ x : ℝ,
        f x =
        x ^ 2 + (18 * x + 30) - 2 * √(x ^ 2 + 18 * x + 45))
    (h₁ : Fintype (↑(f ⁻¹' {0}) : Type)) :
    ∏ x ∈ (f ⁻¹' {0}).toFinset, x = 20 := by
  have h2 : ∀ x : ℝ, f x = 0 ↔ x = -9 + √61 ∨ x = -9 - √61 := by
    intro x
    constructor
    · -- Assume f(x) = 0, prove x = -9 ± √61
        intro hx
        have hfx : f x = x ^ 2 + (18 * x + 30) - 2 * √(x ^ 2 + 18 * x + 45)  := by
          sorry
        rw [hfx] at hx
        have h_eq : x ^ 2 + (18 * x + 30) - 2 * √(x ^ 2 + 18 * x + 45) = 0  := by
          sorry
        have h1 : 2 * √(x ^ 2 + 18 * x + 45) = x ^ 2 + 18 * x + 30  := by
          linarith
        have h2 : x ^ 2 + 18 * x + 45 ≥ 0 := by
            nlinarith [Real.sqrt_nonneg (x ^ 2 + 18 * x + 45)]
        have h3 : √(x ^ 2 + 18 * x + 45) ≥ 0  := by
          sorry
        have h4 : x ^ 2 + 18 * x + 30 ≥ 0  := by
          nlinarith
        have h5 : x ^ 2 + 18 * x + 30 = 2 * √(x ^ 2 + 18 * x + 45)  := by
          linarith
        have h6 : (x ^ 2 + 18 * x + 30) ^ 2 = 4 * (x ^ 2 + 18 * x + 45) := by
            have hsq : (2 * √(x ^ 2 + 18 * x + 45)) ^ 2 = 4 * (x ^ 2 + 18 * x + 45) := by
              sorry
            rw [← h5] at hsq
            nlinarith
        have h7 : (x - (-9 + √61)) * (x - (-9 - √61)) = 0 := by
          sorry
        cases' (mul_eq_zero.mp h7) with h8 h9
        · left
          linarith
        · right
          linarith
    · -- Assume x = -9 ± √61, prove f(x) = 0
        rintro (h | h)
        ·
          sorry
        · rw [h]
          have h1 : √61 > 0  := by
            sorry
          sorry
  sorry
```

## Auto Solver (ProofRepairer)

### Auto Solver Result

```lean
import Mathlib
set_option maxHeartbeats 0
open BigOperators Real Nat Topology Rat
lemma aime_1983_p3_1_1
    (f : ℝ → ℝ)
    (h₀ : ∀ x : ℝ,
        f x =
        x ^ 2 + (18 * x + 30) - 2 * √(x ^ 2 + 18 * x + 45))
    (h₁ : Fintype (↑(f ⁻¹' {0}) : Type)) :
    ∏ x ∈ (f ⁻¹' {0}).toFinset, x = 20 := by
  have h2 : ∀ x : ℝ, f x = 0 ↔ x = -9 + √61 ∨ x = -9 - √61 := by
    intro x
    constructor
    · -- Assume f(x) = 0, prove x = -9 ± √61
        intro hx
        have hfx : f x = x ^ 2 + (18 * x + 30) - 2 * √(x ^ 2 + 18 * x + 45)  := by
          sorry
        rw [hfx] at hx
        have h_eq : x ^ 2 + (18 * x + 30) - 2 * √(x ^ 2 + 18 * x + 45) = 0  := by
          sorry
        have h1 : 2 * √(x ^ 2 + 18 * x + 45) = x ^ 2 + 18 * x + 30  := by
          linarith
        have h2 : x ^ 2 + 18 * x + 45 ≥ 0 := by
            nlinarith [Real.sqrt_nonneg (x ^ 2 + 18 * x + 45)]
        have h3 : √(x ^ 2 + 18 * x + 45) ≥ 0  := by
          sorry
        have h4 : x ^ 2 + 18 * x + 30 ≥ 0  := by
          nlinarith
        have h5 : x ^ 2 + 18 * x + 30 = 2 * √(x ^ 2 + 18 * x + 45)  := by
          linarith
        have h6 : (x ^ 2 + 18 * x + 30) ^ 2 = 4 * (x ^ 2 + 18 * x + 45) := by
            have hsq : (2 * √(x ^ 2 + 18 * x + 45)) ^ 2 = 4 * (x ^ 2 + 18 * x + 45) := by
              sorry
            rw [← h5] at hsq
            nlinarith
        have h7 : (x - (-9 + √61)) * (x - (-9 - √61)) = 0 := by
          sorry
        cases' (mul_eq_zero.mp h7) with h8 h9
        · left
          linarith
        · right
          linarith
    · -- Assume x = -9 ± √61, prove f(x) = 0
        rintro (h | h)
        ·
          sorry
        · rw [h]
          have h1 : √61 > 0  := by
            sorry
          sorry
  sorry
```

## Final Verification

- **Pass:** Yes
- **Complete:** No
## RAG Retrieval Analysis

**Found 9 sorry(s)**

### Sorry #1 (Line 17)

#### Query

```lean
f : ℝ → ℝ
h₀ : ∀ (x : ℝ), f x = x ^ 2 + (18 * x + 30) - 2 * √(x ^ 2 + 18 * x + 45)
h₁ : Fintype ↑(f ⁻¹' {0})
x : ℝ
hx : f x = 0
⊢ f x = x ^ 2 + (18 * x + 30) - 2 * √(x ^ 2 + 18 * x + 45)
```

### Sorry #2 (Line 20)

#### Query

```lean
f : ℝ → ℝ
h₀ : ∀ (x : ℝ), f x = x ^ 2 + (18 * x + 30) - 2 * √(x ^ 2 + 18 * x + 45)
h₁ : Fintype ↑(f ⁻¹' {0})
x : ℝ
hx : x ^ 2 + (18 * x + 30) - 2 * √(x ^ 2 + 18 * x + 45) = 0
hfx : f x = x ^ 2 + (18 * x + 30) - 2 * √(x ^ 2 + 18 * x + 45)
⊢ x ^ 2 + (18 * x + 30) - 2 * √(x ^ 2 + 18 * x + 45) = 0
```

### Sorry #3 (Line 26)

#### Query

```lean
f : ℝ → ℝ
h₀ : ∀ (x : ℝ), f x = x ^ 2 + (18 * x + 30) - 2 * √(x ^ 2 + 18 * x + 45)
h₁ : Fintype ↑(f ⁻¹' {0})
x : ℝ
hx : x ^ 2 + (18 * x + 30) - 2 * √(x ^ 2 + 18 * x + 45) = 0
hfx : f x = x ^ 2 + (18 * x + 30) - 2 * √(x ^ 2 + 18 * x + 45)
h_eq : x ^ 2 + (18 * x + 30) - 2 * √(x ^ 2 + 18 * x + 45) = 0
h1 : 2 * √(x ^ 2 + 18 * x + 45) = x ^ 2 + 18 * x + 30
h2 : x ^ 2 + 18 * x + 45 ≥ 0
⊢ √(x ^ 2 + 18 * x + 45) ≥ 0
```

### Sorry #4 (Line 33)

#### Query

```lean
f : ℝ → ℝ
h₀ : ∀ (x : ℝ), f x = x ^ 2 + (18 * x + 30) - 2 * √(x ^ 2 + 18 * x + 45)
h₁ : Fintype ↑(f ⁻¹' {0})
x : ℝ
hx : x ^ 2 + (18 * x + 30) - 2 * √(x ^ 2 + 18 * x + 45) = 0
hfx : f x = x ^ 2 + (18 * x + 30) - 2 * √(x ^ 2 + 18 * x + 45)
h_eq : x ^ 2 + (18 * x + 30) - 2 * √(x ^ 2 + 18 * x + 45) = 0
h1 : 2 * √(x ^ 2 + 18 * x + 45) = x ^ 2 + 18 * x + 30
h2 : x ^ 2 + 18 * x + 45 ≥ 0
h3 : √(x ^ 2 + 18 * x + 45) ≥ 0
h4 : x ^ 2 + 18 * x + 30 ≥ 0
h5 : x ^ 2 + 18 * x + 30 = 2 * √(x ^ 2 + 18 * x + 45)
⊢ (2 * √(x ^ 2 + 18 * x + 45)) ^ 2 = 4 * (x ^ 2 + 18 * x + 45)
```

### Sorry #5 (Line 37)

#### Query

```lean
f : ℝ → ℝ
h₀ : ∀ (x : ℝ), f x = x ^ 2 + (18 * x + 30) - 2 * √(x ^ 2 + 18 * x + 45)
h₁ : Fintype ↑(f ⁻¹' {0})
x : ℝ
hx : x ^ 2 + (18 * x + 30) - 2 * √(x ^ 2 + 18 * x + 45) = 0
hfx : f x = x ^ 2 + (18 * x + 30) - 2 * √(x ^ 2 + 18 * x + 45)
h_eq : x ^ 2 + (18 * x + 30) - 2 * √(x ^ 2 + 18 * x + 45) = 0
h1 : 2 * √(x ^ 2 + 18 * x + 45) = x ^ 2 + 18 * x + 30
h2 : x ^ 2 + 18 * x + 45 ≥ 0
h3 : √(x ^ 2 + 18 * x + 45) ≥ 0
h4 : x ^ 2 + 18 * x + 30 ≥ 0
h5 : x ^ 2 + 18 * x + 30 = 2 * √(x ^ 2 + 18 * x + 45)
h6 : (x ^ 2 + 18 * x + 30) ^ 2 = 4 * (x ^ 2 + 18 * x + 45)
⊢ (x - (-9 + √61)) * (x - (-9 - √61)) = 0
```

### Sorry #6 (Line 46)

#### Query

```lean
case mpr.inl
f : ℝ → ℝ
h₀ : ∀ (x : ℝ), f x = x ^ 2 + (18 * x + 30) - 2 * √(x ^ 2 + 18 * x + 45)
h₁ : Fintype ↑(f ⁻¹' {0})
x : ℝ
h : x = -9 + √61
⊢ f x = 0
```

### Sorry #7 (Line 49)

#### Query

```lean
f : ℝ → ℝ
h₀ : ∀ (x : ℝ), f x = x ^ 2 + (18 * x + 30) - 2 * √(x ^ 2 + 18 * x + 45)
h₁ : Fintype ↑(f ⁻¹' {0})
x : ℝ
h : x = -9 - √61
⊢ √61 > 0
```

### Sorry #8 (Line 50)

#### Query

```lean
case mpr.inr
f : ℝ → ℝ
h₀ : ∀ (x : ℝ), f x = x ^ 2 + (18 * x + 30) - 2 * √(x ^ 2 + 18 * x + 45)
h₁ : Fintype ↑(f ⁻¹' {0})
x : ℝ
h : x = -9 - √61
h1 : √61 > 0
⊢ f (-9 - √61) = 0
```

### Sorry #9 (Line 51)

#### Query

```lean
f : ℝ → ℝ
h₀ : ∀ (x : ℝ), f x = x ^ 2 + (18 * x + 30) - 2 * √(x ^ 2 + 18 * x + 45)
h₁ : Fintype ↑(f ⁻¹' {0})
h2 : ∀ (x : ℝ), f x = 0 ↔ x = -9 + √61 ∨ x = -9 - √61
⊢ ∏ x ∈ (f ⁻¹' {0}).toFinset, x = 20
```

